VProg/Vprop.v
@@ -250,323 +250,908 @@ Module CTX.
       + apply SLprop.star_comm12.
   Qed.
 
-  Section Trf.
-    Variable (c0 c1 : CTX.t) (rev_f : Sub.t c1 -> (Sub.t c0 * CTX.t (* rem *))).
-    Local Set Implicit Arguments.
+  Module Trf.
+    Section Trf.
+      Variables c0 c1 : CTX.t.
+      Definition rev_f_t := Sub.t c1 -> (Sub.t c0 * CTX.t (* rem *)).
 
-    Record trf : Prop := {
-      trf_fwd : SLprop.imp (sl c0) (sl c1);
-      trf_bwd : forall s1 : Sub.t c1, let r := rev_f s1 in
-                SLprop.imp (sl (sub c1 s1)) (sl (sub c0 (fst r)) ** sl (snd r))
-    }.
-  End Trf.
-  Global Arguments trf : clear implicits.
+      Local Set Implicit Arguments.
+      Record p (rev_f : rev_f_t) : Prop := {
+        fwd : SLprop.imp (sl c0) (sl c1);
+        bwd : forall s1 : Sub.t c1, let (s0, rem) := rev_f s1 in
+              SLprop.imp (sl_sub c1 s1) (sl_sub c0 s0 ** sl rem)
+      }.
 
-  Module Inj.
-    Inductive ieq (c0 c1 : CTX.t) (img : Sub.t c1) :=
-      ieqI (E : SLprop.eq (sl (sub c1 img)) (sl c0)).
+      Definition t : Type := {rev_f : rev_f_t | p rev_f}.
 
-    Lemma ieqE [c0 c1 img] (IEQ : ieq c0 c1 img):
-      SLprop.eq (sl (sub c1 img)) (sl c0).
-    Proof. apply IEQ. Qed.
-
-    Definition beq (c0 c1 : CTX.t) :=
-      ieq c0 c1 (Sub.const c1 true).
-
-    Lemma beq_iff c0 c1:
-      beq c0 c1 <-> SLprop.eq (sl c1) (sl c0).
-    Proof.
-      etransitivity.
-      - split. intros [H]; exact H. intro H; constructor; exact H.
-      - rewrite Sub.sub_const_true. reflexivity.
-    Qed.
-
-    Lemma beqE [c0 c1] (BEQ : beq c0 c1):
-      SLprop.eq (sl c1) (sl c0).
-    Proof.
-      apply beq_iff, BEQ.
-    Qed.
-
-    Definition itrf (c0 c1 : CTX.t) (add : CTX.t) (rev_f : Sub.t (c0 ++ add) -> (Sub.t c1 * CTX.t)) : Prop :=
-      trf c1 (c0 ++ add) rev_f.
-
-    (* Tactic to build an [ieq].
-       We solve goals of the form:
-
-         ieq [mka vp0 ?sel0 ; ... ; mka vp9 ?sel5 ]
-             [mka vp0' sel0'; ... ; mka vp9' sel9']
-             ?img
-
-       and instantiate [?sel0]...[?sel5] and [?img] in the process.
-       To do so, we find an ordered subset of [c1] that matches [c0].
-    *)
-
-    (* An ordered subset is described by associating an index (order) to the elements of the subset. *)
-    Definition osub (c1 : CTX.t) := Vector.t (option nat) (length c1).
-
-    Section OSub_IEq.
-      Fixpoint n_insert (n : nat) (x : atom) (xs : list (nat * atom)) : list (nat * atom) :=
-        match xs with
-        | nil => [(n, x)]
-        | (n', x') :: tl => if Nat.leb n n' then (n, x) :: xs
-                            else (n', x') :: n_insert n x tl
-        end.
-
-      Lemma n_insert_eq n x xs:
-        SLprop.eq (sl (map snd (n_insert n x xs))) (sla x ** sl (map snd xs)).
+      Lemma t_fwd (p : t) : SLprop.imp (sl c0) (sl c1).
       Proof.
-        revert n x; induction xs as [|(n', x') tl]; intros; simpl.
-        - reflexivity.
-        - case Nat.leb; simpl.
-          + reflexivity.
-          + rewrite IHtl, SLprop.star_comm12; reflexivity.
+        case p as [? [fwd _]].
+        exact fwd.
       Qed.
+    End Trf.
+    Global Arguments Trf.p : clear implicits.
 
-      Fixpoint n_list_of_osub (c1 : CTX.t) : osub c1 -> list (nat * atom).
+    Definition inj_p (c0 c1 add : CTX.t) (rev_f : rev_f_t c0 (c1 ++ add)) : Prop :=
+      Trf.p c0 (c1 ++ add) rev_f.
+
+    Section Refl.
+      Variable c : CTX.t.
+      
+      Definition refl_rev_f : rev_f_t c c :=
+        fun s => (s, nil).
+
+      Lemma refl_p : Trf.p c c refl_rev_f.
       Proof.
-        case c1 as [|a c1].
-        - intros _. exact nil.
-        - intros [[n|] sb]%Vector.uncons.
-          + exact (n_insert n a (n_list_of_osub c1 sb)).
-          + exact (n_list_of_osub c1 sb).
-      Defined.
-
-      (* [c0 : CTX.t] and [img] associated to an ordered subset. *)
-      Definition c0_of_osub (c1 : CTX.t) (sb : osub c1) : CTX.t :=
-        map snd (n_list_of_osub c1 sb).
-
-      Global Arguments c0_of_osub _ !_/.
-
-      Definition img_of_osub (c1 : CTX.t) : osub c1 -> Sub.t c1 :=
-        Vector.map (fun o => match o with Some _ => true | None => false end).
-
-      (* By construction, the [ieq] relation is satisfied. *)
-      Lemma osub_ieq (c1 : CTX.t) (sb : osub c1):
-        ieq (c0_of_osub c1 sb) c1 (img_of_osub c1 sb).
-      Proof.
-        constructor; induction c1.
-        - simpl; reflexivity.
-        - case sb as [[]] using Vector.caseS'; simpl.
-          + rewrite n_insert_eq.
-            apply SLprop.star_morph_eq. reflexivity.
-            apply IHc1.
-          + apply IHc1.
+        split; cbn; intros; SL.normalize; reflexivity.
       Qed.
-    End OSub_IEq.
+    End Refl.
+    Section Trans.
+      Context [c0 c1 c2 : CTX.t] (f0 : rev_f_t c0 c1) (f1 : rev_f_t c1 c2).
 
-    (* Alternatively We can also build a [trf] *)
-    Section OSub_Trf.
-      Definition nat_opt_le (n0 n1 : option nat) : bool :=
-        match n1, n0 with
-        | None,    _       => true
-        | Some n1, Some n0 => Nat.leb n0 n1
-        | Some _,  None    => false
-        end.
+      Definition trans_rev_f : rev_f_t c0 c2 :=
+        fun s2 => let (s1, rem1) := f1 s2 in
+                  let (s0, rem0) := f0 s1 in
+                  (s0, rem0 ++ rem1).
 
-      Fixpoint trf_insert (n : option nat) (x : atom) (l : list (option nat * atom)) {struct l}:
-        { l' : list (option nat * atom) & Sub.t (List.map snd l') -> Sub.t (x :: List.map snd l) }.
+      Lemma trans_p (T0 : Trf.p c0 c1 f0) (T1 : Trf.p c1 c2 f1) : Trf.p c0 c2 trans_rev_f.
       Proof.
-        case l as [|(n', x') l].
-        - exists [(n,x)].
-          exact (fun s => s).
-        - case (nat_opt_le n n').
-          + exists ((n, x) :: (n', x') :: l).
-            exact (fun s => s).
-          + case (trf_insert n x l) as [l' f].
-            exists ((n', x') :: l').
-            intros [b' [b bl]%f%Vector.uncons]%Vector.uncons.
-            exact (Vector.cons _ b _ (Vector.cons _ b' _ bl)).
-      Defined.
-
-      Lemma trf_insert_correct n x l:
-        let '(existT _ l' f) := trf_insert n x l in
-        SLprop.eq (sl (x :: map snd l)) (sl (map snd l')) /\
-        forall s, SLprop.eq (sl_sub (map snd l') s) (sl_sub (x :: map snd l) (f s)).
-      Proof.
-        induction l as [|(n', x') l IH]; cbn; [|case nat_opt_le]; cbn.
-        1,2:split; reflexivity.
-        destruct trf_insert as [l' f]; cbn; split.
-        - rewrite <- (proj1 IH); cbn.
-          apply SLprop.star_comm12.
-        - intro s.
-          rewrite (proj2 IH); cbn.
-          apply SLprop.star_comm12.
-      Qed.
-
-      Fixpoint trf_sort_list (c1 : CTX.t) { struct c1 } :
-        forall sb : osub c1,
-        { l : list (option nat * atom) & Sub.t (List.map snd l) -> Sub.t c1 }.
-      Proof.
-        case c1 as [|x c1].
-        - exact (fun _ => existT _ nil (fun _ => Vector.nil _)).
-        - intros (n, sb)%Vector.uncons.
-          case (trf_sort_list c1 sb) as [l0 f0].
-          case (trf_insert   n x l0) as [l1 f1].
-          exists l1.
-          exact (fun s1 => let (b, s0) := Vector.uncons (f1 s1) in Vector.cons _ b _ (f0 s0)).
-      Defined.
-
-      Lemma trf_sort_list_correct c1 sb:
-        let '(existT _ l' f) := trf_sort_list c1 sb in
-        SLprop.eq (sl c1) (sl (map snd l')) /\
-        forall s, SLprop.eq (sl_sub (map snd l') s) (sl_sub c1 (f s)).
-      Proof.
-        induction c1 as [|x c1 IH]; cbn.
-        - split; reflexivity.
-        - case sb as [n sb] using Vector.caseS'; cbn.
-          specialize (IH sb).
-          destruct trf_sort_list as [l0 f0].
-          specialize (trf_insert_correct n x l0) as IC.
-          destruct trf_insert    as [l1 f1].
-          split.
-          + rewrite <- (proj1 IC); cbn.
-            rewrite <- (proj1 IH); reflexivity.
-          + intro s; cbn.
-            rewrite (proj2 IC); cbn.
-            rewrite (proj2 IH); reflexivity.
-      Qed.
-
-      Variables (c1 : CTX.t) (sb : osub c1).
-
-      Definition trf_c0_of_osub : CTX.t :=
-        List.map snd (projT1 (trf_sort_list c1 sb)).
-
-      Definition trf_rev_f_of_osub (s : Sub.t trf_c0_of_osub) : Sub.t c1 * CTX.t :=
-        (projT2 (trf_sort_list c1 sb) s, nil).
-
-      Lemma osub_trf:
-        trf c1 trf_c0_of_osub trf_rev_f_of_osub.
-      Proof.
-        unfold trf_rev_f_of_osub, trf_c0_of_osub.
-        specialize (trf_sort_list_correct c1 sb).
-        pattern (trf_sort_list c1 sb).
-        destruct trf_sort_list as [c0 f]; cbn.
-        intros [FWD BWD].
         split.
-        - rewrite FWD; reflexivity.
-        - intro s; cbn.
-          rewrite !sl_sub_eq, BWD.
-          SL.normalize.
-          reflexivity.
+        - rewrite (fwd T0), (fwd T1); reflexivity.
+        - unfold trans_rev_f; intro s2.
+          specialize (bwd T1 s2); case f1 as (s1, rem1).
+          specialize (bwd T0 s1); case f0 as (s0, rem0).
+          cbn; intros E0 ->.
+          etransitivity. { apply SLprop.star_morph_imp. exact E0. reflexivity. }
+          rewrite sl_app; SL.normalize; reflexivity.
       Qed.
-    End OSub_Trf.
+    End Trans.
+    Section Atom.
+      Definition atomt (rev : bool) (c0 c1 : CTX.t) :=
+        if rev
+        then SLprop.eq  (sl c0) (sl c1)
+        else SLprop.imp (sl c0) (sl c1).
 
-
-    (* To find an ordered subset of [c1] that matches [c0], we generate a dummy goal:
-
-         H9 : ieq_asm (mka vp9' sel9') ?n9
-           ...
-         H0 : ieq_asm (mka vp0' sel0') ?n0
-         ===============================================
-         ieq_goal k [mka vp0 ?sel0; ... ; mka vp5 ?sel5]
-
-       We than consider the elements of [c0] in sequence.
-       For each atom [mka vp_i ?sel_i], we find a matching [ieq_asm (mka vp_j' sel_j') ?n_j]
-       (with [vp_j' = vp_i]).
-       We set [?sel_i] to [sel_j'] and [?n_j] to the current position [k] in [c0].
-       We pop [mka vp_i _] from [c0], removes [ieq_asm (mka vp_j' sel_j') _] from the hypotheses,
-       increments [k] and continue with the next atom of [c0].
-       When [c0] becomes empty, we assign [None] to all remaining [ieq_asm].
-     *)
-
-    Inductive ieq_asm (a : atom) (n : option nat): Prop :=.
-
-    Local Lemma inst_ieq_asm a : ieq_asm a None -> unit.
-    Proof. constructor. Qed.
-
-    Global Ltac clear_ieq_asm :=
-      repeat lazymatch goal with
-      | H : ieq_asm _ ?n |- _ => apply inst_ieq_asm in H; clear H
-      end.
-
-    Inductive ieq_goal : forall (n : nat) (c0 : CTX.t), Prop :=
-      | Ieq_Done n : ieq_goal n nil
-      | Ieq_Cons [n a c0] (A : ieq_asm a (Some n)) (C : ieq_goal (S n) c0) : ieq_goal n (a :: c0).
-
-    (* NOTE: we reverse the order of [c1] so that the most recent hypotheses (which are chosen by the
-       [match] in case of multiple possibilities) are the leftmost atoms. *)
-    Fixpoint ieq_unification_goal_aux (TRG : Prop) (c1 : CTX.t): forall (sb : osub c1), Prop.
-    Proof.
-      case c1 as [|a c1].
-      - intros _; exact TRG.
-      - intros [n sb]%Vector.uncons.
-        exact (ieq_unification_goal_aux (ieq_asm a n -> TRG) c1 sb).
-    Defined.
-    
-    Definition ieq_unification_goal (c0 c1 : CTX.t) (sb : osub c1): Prop :=
-      ieq_unification_goal_aux (ieq_goal O c0) c1 sb.
-
-    (* solves a goal [ieq_unification_goal c0 c1 ?sb] *)
-    Ltac build_ieq_unification_goal :=
-      clear; cbn; intros;
-      repeat lazymatch goal with
-      | H : CTX.Inj.ieq_asm (existT _ ?v _) _ |- CTX.Inj.ieq_goal _ (existT _ ?v _ :: _) =>
-          refine (Ieq_Cons H _); clear H
-      | |- ieq_goal _ nil =>
-          clear_ieq_asm; exact (Ieq_Done _)
-      | |- ieq_goal _ (existT _ ?v _ :: _) =>
-          idtac "FAILURE: Inj.build failed to find" v ". Remaining context:";
-          try match goal with
-           _ : CTX.Inj.ieq_asm (existT _ ?v0 _) _ |- _ => idtac "-" v0; fail
-          end;
-          fail 1 "Inj.build" v
-      end.
-
-    Local Lemma build_ieq_by_osub [c0 c1 : CTX.t]
-      (sb : osub c1)
-      (U  : ieq_unification_goal c0 c1 sb)
-      (C0 : c0 = c0_of_osub c1 sb)
-      [img : Sub.t c1] (IMG : img = img_of_osub c1 sb):
-      ieq c0 c1 img.
-    Proof.
-      subst; apply osub_ieq.
-    Qed.
-
-    (* solves a goal [ieq c0 c1 img]
-       The selectors of [c0] must be evars.
-       [img] can be an evar. *)
-    Global Ltac build_ieq :=
-      simple refine (build_ieq_by_osub _ _ _ _);
-      [ (* sb  *) Vector.build_shape
-      | (* U   *) build_ieq_unification_goal  
-      | (* C0  *) cbn; reflexivity
-      | (* IMG *) cbn; reflexivity ].
-
-    (* This builds an injection then checks that it consumes everything. *)
-    Global Ltac build_beq := build_ieq.
-
-    Local Lemma build_itrf_by_osub [c0 c1 : CTX.t]
-      (sb : osub c1)
-      (U : ieq_unification_goal c0 c1 sb)
-      [add : CTX.t] (C0 : c0 ++ add = trf_c0_of_osub c1 sb):
-      itrf c0 c1 add (eq_rect_r (fun c0a => Sub.t c0a -> _) (trf_rev_f_of_osub c1 sb) C0).
-    Proof.
-      unfold itrf.
-      specialize (osub_trf c1 sb).
-      generalize (trf_rev_f_of_osub c1 sb) as rev_f.
-      case C0; cbn.
-      auto.
-    Qed.
-
-    (* solves a goal [itrf c0 c1 ?add ?rev_f]
-       The selectors of [c0] must be evars. *)
-    Global Ltac build_itrf :=
-      simple refine (build_itrf_by_osub _ _ _);
-      [ (* sb *) Vector.build_shape
-      | (* U  *) build_ieq_unification_goal
-      | (* C0 *) cbn; reflexivity ].
-
-    Section Test.
-      Variable v : nat -> Vprop.p nat.
-
-      Goal exists sl0 sl1 add rev_f,
-        itrf [mka (v 0, sl0); mka (v 1, sl1)] [mka (v 1, 1); mka (v 2, 2); mka (v 0, 0)]
-          add rev_f.
+      Lemma atom_imp [rev c0 c1] (T : atomt rev c0 c1) : SLprop.imp (sl c0) (sl c1).
       Proof.
-        do 4 eexists. build_itrf.
+        destruct rev; cbn in T; rewrite T; reflexivity.
       Qed.
-    End Test.
-  End Inj.
+
+      Definition atom_rev_f (rev : bool) (c0 c1 : CTX.t) : rev_f_t c0 c1 :=
+        fun s1 =>
+        if andb rev (Vector.allb s1)
+        then (Vector.const true  (length c0), nil)
+        else (Vector.const false (length c0), CTX.sub c1 s1).
+
+      Lemma atom_p [rev c0 c1] (T : atomt rev c0 c1) : Trf.p c0 c1 (atom_rev_f rev c0 c1).
+      Proof.
+        split.
+          { apply (atom_imp T). }
+        intro s1.
+        destruct rev; unfold atom_rev_f; cbn in *;
+          [case (BoolSpec_of_iff (Vector.allb_iff_const s1)) as [->|_]|]; cbn.
+        2,3:rewrite <-!sl_sub_eq, Sub.sub_const_false; SL.normalize; reflexivity.
+        rewrite <-!sl_sub_eq, !Sub.sub_const_true, T; SL.normalize; reflexivity.
+      Qed.
+    End Atom.
+    Section Cons. 
+      Variables (a : CTX.atom) (c0 c1 : CTX.t) (f : rev_f_t c0 c1).
+
+      Definition cons_rev_f : rev_f_t (a :: c0) (a :: c1) :=
+        fun s1 =>
+        let (b,   s1) := Vector.uncons (n := length c1) s1 in
+        let (s0, rem) := f s1 in
+        (Vector.cons _ b (length c0) s0, rem).
+
+      Lemma cons_p (T : Trf.p c0 c1 f) : Trf.p (a :: c0) (a :: c1) cons_rev_f.
+      Proof.
+        split.
+        - apply SLprop.star_morph_imp. reflexivity. exact (fwd T).
+        - intro s1; case s1 as [b s1] using Vector.caseS'; cbn.
+          specialize (bwd T s1); case (f s1) as (s0, rem); cbn; intro E.
+          SL.normalize.
+          eapply SLprop.star_morph_imp. reflexivity.
+          exact E.
+      Qed.
+    End Cons.
+    Section Swap.
+      Context (a0 a1 : CTX.atom) [c0 c1 : CTX.t] (f : rev_f_t c0 c1).
+
+      Definition swap_rev_f : rev_f_t (a0 :: a1 :: c0) (a1 :: a0 :: c1) :=
+        fun s1 =>
+        let (b1,  s1) := Vector.uncons (n := S (length c1)) s1 in
+        let (b0,  s1) := Vector.uncons (n :=    length c1 ) s1 in
+        let (s0, rem) := f s1 in
+        (Vector.cons _ b0 (S (length c0)) (Vector.cons _ b1 (length c0) s0), rem).
+
+      Lemma swap_p (T : Trf.p c0 c1 f) : Trf.p (a0 :: a1 :: c0) (a1 :: a0 :: c1) swap_rev_f.
+      Proof.
+        split.
+        - cbn; rewrite SLprop.star_comm12.
+          do 2 (apply SLprop.star_morph_imp; [reflexivity|]).
+          exact (fwd T).
+        - intro s1;
+            case s1 as [b1 s1] using Vector.caseS';
+            case s1 as [b0 s1] using Vector.caseS';
+            cbn.
+          specialize (bwd T s1); case (f s1) as (s0, rem); cbn; intro E.
+          rewrite SLprop.star_comm12; SL.normalize.
+          do 2 (eapply SLprop.star_morph_imp; [reflexivity|]).
+          exact E.
+      Qed.
+    End Swap.
+    Section App.
+      Context [ca0 ca1 : CTX.t] (fa : rev_f_t ca0 ca1)
+              [cb0 cb1 : CTX.t] (fb : rev_f_t cb0 cb1).
+
+      Definition app_rev_f : rev_f_t (ca0 ++ cb0) (ca1 ++ cb1)
+        := fun s1 =>
+        let (s1a, s1b) := Sub.split ca1 cb1 s1 in
+        let (s0a, rea) := fa s1a in
+        let (s0b, reb) := fb s1b in
+        (Sub.app s0a s0b, rea ++ reb).
+
+      Lemma app_p (Ta : Trf.p ca0 ca1 fa) (Tb : Trf.p cb0 cb1 fb)
+        : Trf.p (ca0 ++ cb0) (ca1 ++ cb1) app_rev_f.
+      Proof.
+        split.
+        - rewrite !sl_app.
+          apply SLprop.star_morph_imp.
+          + apply Ta.
+          + apply Tb.
+        - intro s1; unfold app_rev_f.
+          specialize (Sub.app_split ca1 cb1 s1).
+          case Sub.split as (s1a, s1b).
+          specialize (bwd Tb s1b); specialize (bwd Ta s1a).
+          case fa as (s0a, rea), fb as (s0b, reb).
+          cbn; intros Ea Eb ->.
+          rewrite <-!sl_sub_eq, !Sub.sub_app, !sl_app, !sl_sub_eq.
+          etransitivity.
+          + apply SLprop.star_morph_imp. exact Ea. exact Eb.
+          + SL.normalize.
+            setoid_rewrite SLprop.star_comm12 at 2.
+            reflexivity.
+      Qed.
+    End App.
+
+    Module Tac.
+      (* Tactic to build a [Trf.p] or a [Trf.inj_p] *)
+
+      Definition elim_rule (rev : bool) (a : atom) (r : CTX.t) :=
+        atomt rev [a] r.
+
+      (* [PT] and [PF] must be propositions solvable using [split] (typically equalities).
+         [PT] is enforced when the transformation is committed and should define the selector of
+         [a] from the selectors of [r].
+         [PF] is enforced when the transformation is cancelled and should define the selectors of
+         [r] from the selector of [a]. *)
+      Record intro_rule (rev : bool) (a : atom) (r : CTX.t) (PT PF : Prop) : Prop := mk_intro_rule {
+        get_intro_rule : forall (E : PT), atomt rev r [a]
+      }.
+      Global Arguments get_intro_rule [_ _ _ _ _].
+
+      Definition unfold_rule (a b : atom) := a = b.
+
+      (* Database for automatic introduction/elimination rules.
+         Called on goals:
+           [elim_rule ?rev a ?r]
+           [intro_rule ?rev a ?r ?PT ?PF]
+           [unfold_rule a ?b]
+       *)
+      Global Create HintDb CtxTrfDB discriminated.
+      Global Hint Constants Opaque : CtxTrfDB.
+      Global Hint Variables Opaque : CtxTrfDB.
+
+      Definition ord_t := option (list nat).
+
+      Definition ord_le (i0 i1 : ord_t) : bool :=
+        match i1, i0 with
+        | None,    _       => true
+        | Some _,  None    => false
+        | Some l1, Some l0 =>
+            (fix cmp_list l0 l1 {struct l0} :=
+             match l0, l1 with
+             | x0 :: l0, x1 :: l1 =>
+                 match Nat.compare x0 x1 with
+                 | Lt => true
+                 | Gt => false
+                 | Eq => cmp_list l0 l1
+                 end
+             | nil, nil => true
+             | _,   _   => true (* placeholder *)
+             end) l0 l1
+        end.
+
+      Section WitA.
+        Inductive wit_A : CTX.atom -> Type :=
+          | WitAAtom (i : ord_t) (a : atom) : wit_A a
+          | WitATrf [rev : bool] [a : atom] [r : CTX.t] (T : Trf.atomt rev [a] r)
+              (C : ForallT wit_A r) : wit_A a.
+
+        Definition wit_Al0_res
+          (R : forall (a : atom) (w : wit_A a), list (ord_t * atom))
+          [r : CTX.t] (C : ForallT wit_A r) : list (ord_t * atom) :=
+          concat (ForallT_join R r C).
+        Fixpoint wit_A_res [a : atom] (w : wit_A a) {struct w} : list (ord_t * atom) :=
+          match w with
+          | WitAAtom a i => [(a, i)]
+          | WitATrf _ C  => wit_Al0_res (@wit_A_res) C
+          end.
+        Definition wit_Al_res [r] C := @wit_Al0_res (@wit_A_res) r C.
+
+        Definition wit_Al0_rev_f
+          (R : forall (a : atom) (w : wit_A a), rev_f_t [a] (map snd (wit_A_res w)))
+          : forall [r : CTX.t] (C : ForallT wit_A r),
+          rev_f_t r (map snd (wit_Al_res C)).
+        Proof.
+          fix rc 2; intros ? [|a r w C]; cbn.
+          - exact (refl_rev_f nil).
+          - rewrite List.Transp.map_app.
+            exact (app_rev_f (R a w) (rc r C)).
+        Defined.
+        Fixpoint wit_A_rev_f [a : atom] (w : wit_A a) {struct w} : rev_f_t [a] (map snd (wit_A_res w)) :=
+          match w with
+          | WitAAtom i a => refl_rev_f [a]
+          | @WitATrf rev a r T C =>
+              trans_rev_f (atom_rev_f rev [a] r) (@wit_Al0_rev_f (@wit_A_rev_f) r C)
+          end.
+        Definition wit_Al_rev_f [r] C := @wit_Al0_rev_f (@wit_A_rev_f) r C.
+
+        Lemma wit_Al0_trf
+          (R : forall (a : atom) (w : wit_A a), Trf.p [a] (map snd (wit_A_res w)) (wit_A_rev_f w))
+          : forall [r : CTX.t] (C : ForallT wit_A r),
+          Trf.p r (map snd (wit_Al_res C)) (wit_Al_rev_f C).
+        Proof.
+          fix IH 2.
+          intros _ [|a r w C]; cbn.
+          * apply refl_p.
+          * unfold eq_rect_r; case eq_sym; cbn.
+            exact (app_p _ _ (R a w) (IH r C)).
+        Defined.
+        Lemma wit_A_trf [a : atom] (w : wit_A a):
+          Trf.p [a] (map snd (wit_A_res w)) (wit_A_rev_f w).
+        Proof.
+          revert a w; fix IH 2.
+          intros _ [|rev a r T C]; cbn.
+          - apply refl_p.
+          - eapply trans_p.
+            + apply (atom_p T).
+            + exact (wit_Al0_trf IH C).
+        Qed.
+        Definition wit_Al_trf [r] C := @wit_Al0_trf (@wit_A_trf) r C.
+      End WitA.
+      Section WitB.
+        Inductive wit_B : atom -> Type :=
+          | WitBAtom (a : atom) : wit_B a
+          | WitBTrf [rev : bool] [a : atom] [r : CTX.t] (T : Trf.atomt rev r [a])
+              (C : ForallT wit_B r) : wit_B a.
+
+        Definition wit_Bl0_res
+          (R : forall (a : atom) (w : wit_B a), CTX.t)
+          [r : CTX.t] (C : ForallT wit_B r) : CTX.t :=
+          concat (ForallT_join R r C).
+        Fixpoint wit_B_res [a : atom] (w : wit_B a) {struct w} : CTX.t :=
+          match w with
+          | WitBAtom a => [a]
+          | WitBTrf _ C  => wit_Bl0_res (@wit_B_res) C
+          end.
+        Definition wit_Bl_res [r] C := @wit_Bl0_res (@wit_B_res) r C.
+
+        Definition wit_Bl0_rev_f
+          (R : forall (a : atom) (w : wit_B a), rev_f_t (wit_B_res w) [a])
+          : forall [r : CTX.t] (C : ForallT wit_B r),
+          rev_f_t (wit_Bl_res C) r.
+        Proof.
+          fix rc 2; intros ? [|a r w C]; cbn.
+          - exact (refl_rev_f nil).
+          - exact (app_rev_f (R a w) (rc r C)).
+        Defined.
+        Fixpoint wit_B_rev_f [a : atom] (w : wit_B a) {struct w} : rev_f_t (wit_B_res w) [a] :=
+          match w with
+          | WitBAtom a => refl_rev_f [a]
+          | @WitBTrf rev a r T C =>
+              trans_rev_f (@wit_Bl0_rev_f (@wit_B_rev_f) r C) (atom_rev_f rev r [a])
+          end.
+        Definition wit_Bl_rev_f [r] C := @wit_Bl0_rev_f (@wit_B_rev_f) r C.
+
+        Lemma wit_Bl0_trf
+          (R : forall (a : atom) (w : wit_B a), Trf.p (wit_B_res w) [a] (wit_B_rev_f w))
+          : forall [r : CTX.t] (C : ForallT wit_B r),
+          Trf.p (wit_Bl_res C) r (wit_Bl_rev_f C).
+        Proof.
+          fix IH 2.
+          intros _ [|a r w C]; cbn.
+          * apply refl_p.
+          * exact (app_p _ _ (R a w) (IH r C)).
+        Defined.
+        Lemma wit_B_trf [a : atom] (w : wit_B a):
+          Trf.p (wit_B_res w) [a] (wit_B_rev_f w).
+        Proof.
+          revert a w; fix IH 2.
+          intros _ [|rev a r T C]; cbn.
+          - apply refl_p.
+          - eapply trans_p.
+            + exact (wit_Bl0_trf IH C).
+            + apply (atom_p T).
+        Qed.
+        Definition wit_Bl_trf [r] C := @wit_Bl0_trf (@wit_B_trf) r C.
+      End WitB.
+      Section Sort.
+        Fixpoint trf_insert (n : ord_t) (x : atom) (l : list (ord_t * atom)) {struct l}:
+          { l' : list (ord_t * atom) & rev_f_t (x :: List.map snd l) (List.map snd l') }.
+        Proof.
+          case l as [|(n', x') l].
+          - exists [(n,x)].
+            apply refl_rev_f.
+          - case (ord_le n n').
+            + exists ((n, x) :: (n', x') :: l).
+              apply refl_rev_f.
+            + case (trf_insert n x l) as [l' f].
+              exists ((n', x') :: l').
+              eapply trans_rev_f; cbn.
+              * apply swap_rev_f, refl_rev_f.
+              * apply cons_rev_f, f.
+        Defined.
+
+        Lemma trf_insert_correct n x l:
+          let '(existT _ l' f) := trf_insert n x l in
+          Trf.p (x :: map snd l) (map snd l') f.
+        Proof.
+          induction l as [|(n', x') l IH]; cbn; [|case ord_le]; cbn.
+          1,2:split; apply refl_p.
+          destruct trf_insert as [l' f]; cbn.
+          apply trans_p.
+          - apply swap_p, refl_p.
+          - apply cons_p, IH.
+        Qed.
+
+        Fixpoint trf_sort_list (l : list (ord_t * atom)) {struct l} :
+          { l' : list (ord_t * atom) & rev_f_t (List.map snd l) (List.map snd l') }.
+        Proof.
+          case l as [|(n, x) l].
+          - refine (existT _ nil _).
+            apply refl_rev_f.
+          - case (trf_sort_list   l) as [l0 f0].
+            case (trf_insert n x l0) as [l1 f1].
+            exists l1.
+            eapply trans_rev_f.
+            + apply cons_rev_f, f0.
+            + exact f1.
+        Defined.
+
+        Lemma trf_sort_list_correct l:
+          let '(existT _ l' f) := trf_sort_list l in
+          Trf.p (map snd l) (map snd l') f.
+        Proof.
+          induction l as [|(n, x) l IH]; cbn.
+          - apply refl_p.
+          - destruct trf_sort_list as [l0 f0].
+            specialize (trf_insert_correct n x l0) as IC.
+            destruct trf_insert    as [l1 f1].
+            apply trans_p.
+            + apply cons_p, IH.
+            + apply IC.
+        Qed.
+
+        Variable l : list (ord_t * atom).
+
+        Definition trf_sort_res : CTX.t :=
+          map snd (projT1 (trf_sort_list l)).
+
+        Definition trf_sort_rev_f : rev_f_t (map snd l) trf_sort_res :=
+          projT2 (trf_sort_list l).
+
+        Lemma trf_sort_correct:
+          Trf.p (map snd l) trf_sort_res trf_sort_rev_f.
+        Proof.
+          unfold trf_sort_res, trf_sort_rev_f.
+          specialize (trf_sort_list_correct l).
+          destruct trf_sort_list as [res f]; cbn.
+          auto.
+        Qed.
+      End Sort.
+      Section Helpers.
+        Definition rord_t := list nat.
+        Definition ord_of_r (r : rord_t) : ord_t := Some (rev_append r []).
+        Definition ord_None : ord_t := None.
+
+        Inductive state_A (a : atom) :=
+          | StAFirst (wit : wit_A a)
+          | StATrf   (n : ord_t) (committed : option bool).
+        Global Arguments StAFirst [_].
+        Global Arguments StATrf   [_].
+        Inductive A (a : atom) (s : state_A a) (p : list bool) := mk_A.
+
+        Record committed_B_t := mk_cb {
+          cb_PT : Prop;
+          cb_PF : Prop;
+          cb_c  : {cb_PT}+{cb_PF};
+        }.
+        Inductive state_B (a : atom) :=
+          | StBFirst (wit : wit_B a)
+          | StBTrf   (committed : option committed_B_t).
+        Global Arguments StBFirst [_].
+        Global Arguments StBTrf   [_].
+        Inductive B (a : atom) (n : rord_t) (s : state_B a) (p : list committed_B_t) := mk_B.
+
+        Record trf_wit (c0 c1 : CTX.t) := mk_trf_wit {
+          w_witA : ForallT wit_A c0;
+          w_witB : ForallT wit_B c1;
+        }.
+        Global Arguments mk_trf_wit [_ _].
+
+        Definition intro_wit_A (ps : list bool) : Type -> CTX.t -> Type :=
+          List.fold_right (fun a T => {w : wit_A a & A a (StAFirst w) ps -> T}).
+        Fixpoint intro_wit_B (ps : list committed_B_t) (n : nat) (ntl : rord_t)
+          (T : Type) (c1 : CTX.t) {struct c1} : Type :=
+          match c1 with
+          | nil     => T
+          | a :: c1 =>
+              let T := intro_wit_B ps (S n) ntl T c1 in
+              {w : wit_B a & B a (n :: ntl) (StBFirst w) ps -> T}
+          end.
+        Definition intro_wit_trf (c0 c1 : CTX.t) : Type :=
+          intro_wit_B nil O nil (intro_wit_A nil True c0) c1.
+
+        Fixpoint wit_of_intro_A [ps T c0] {struct c0}:
+          forall (W : intro_wit_A ps T c0), ForallT wit_A c0 * T.
+        Proof.
+          case c0 as [|a c0]; cbn.
+          - intro W. split. constructor. exact W.
+          - intros [w W].
+            ecase wit_of_intro_A as [y x]. { apply W. split. }
+            split. constructor.
+            exact w. exact y. exact x.
+        Defined.
+
+        Fixpoint wit_of_intro_B [ps n ntl T c1] {struct c1}:
+          forall (W : intro_wit_B ps n ntl T c1), ForallT wit_B c1 * T.
+        Proof.
+          case c1 as [|a c1]; cbn.
+          - intro W. split. constructor. exact W.
+          - intros [w W].
+            ecase wit_of_intro_B as [y x]. { apply W. split. }
+            split. constructor.
+            exact w. exact y. exact x.
+        Defined.
+
+        Definition wit_of_intro_trf [c0 c1] (W : intro_wit_trf c0 c1) : trf_wit c0 c1 :=
+          let (wB, W) := wit_of_intro_B W in
+          let (wA, _) := wit_of_intro_A W in
+          mk_trf_wit wA wB.
+      End Helpers.
+
+      Local Lemma build_trf_lem (c0 c1 : CTX.t)
+        (W : intro_wit_trf c0 c1)
+        (wA : ForallT wit_A c0) (wB : ForallT wit_B c1)
+        (EW : mk_trf_wit wA wB = wit_of_intro_trf W):
+        let c0_0 := wit_Al_res wA     in
+        let c0_1 := trf_sort_res c0_0 in
+        let c1_0 := wit_Bl_res wB     in
+        forall (E : c1_0 = c0_1),
+        Trf.p c0 c1
+          (@trans_rev_f c0 c0_1 c1 (@trans_rev_f c0 (map snd c0_0) c0_1
+            (wit_Al_rev_f wA)
+            (trf_sort_rev_f c0_0))
+            (eq_rect c1_0 (fun c => rev_f_t c c1) (wit_Bl_rev_f wB) c0_1 E)).
+      Proof.
+        clear W EW.
+        intros c0_0 c0_1 c1_0 E.
+        set (f0 := trans_rev_f _ _) at 2.
+        assert (Trf.p c0 c0_1 f0) as T0. {
+          apply trans_p.
+          - apply wit_Al_trf.
+          - apply trf_sort_correct.
+        }
+        clearbody f0 c0_1; clear c0_0; destruct E; cbn.
+        apply trans_p.
+        - exact T0.
+        - apply wit_Bl_trf.
+      Qed.
+
+      Local Lemma build_inj_lem (c0 c1 add : CTX.t)
+        (W : intro_wit_trf c0 c1)
+        (wA : ForallT wit_A c0) (wB : ForallT wit_B c1)
+        (EW : mk_trf_wit wA wB = wit_of_intro_trf W):
+        let c0_0 := wit_Al_res wA     in
+        let c0_1 := trf_sort_res c0_0 in
+        let c1_0 := wit_Bl_res wB     in
+        forall (E : c1_0 ++ add = c0_1),
+        Trf.inj_p c0 c1 add
+          (@trans_rev_f c0 c0_1 (c1 ++ add) (@trans_rev_f c0 (map snd c0_0) c0_1
+            (wit_Al_rev_f wA)
+            (trf_sort_rev_f c0_0))
+            (eq_rect (c1_0 ++ add) (fun c => rev_f_t c (c1 ++ add))
+              (app_rev_f (wit_Bl_rev_f wB) (refl_rev_f add)) c0_1 E)).
+      Proof.
+        clear W EW.
+        intros c0_0 c0_1 c1_0 E.
+        set (f0 := trans_rev_f _ _) at 2.
+        assert (Trf.p c0 c0_1 f0) as T0. {
+          apply trans_p.
+          - apply wit_Al_trf.
+          - apply trf_sort_correct.
+        }
+        clearbody f0 c0_1; clear c0_0; destruct E; cbn.
+        apply trans_p.
+        - exact T0.
+        - apply app_p.
+          + apply wit_Bl_trf.
+          + apply refl_p.
+      Qed.
+
+      Ltac intro_wit_goal :=
+        cbn;
+        repeat (simple refine (existT _ _ _); [shelve|intro]).
+
+      Ltac commit_parents_A ps :=
+        lazymatch ps with
+        | ?b :: ?ps =>
+            tryif is_evar b
+            then (unify b true; commit_parents_A ps)
+            else idtac
+        | nil => idtac
+        end.
+ 
+      Ltac commit_parents_B ps :=
+        lazymatch ps with
+        | mk_cb _ _ ?c :: ?ps =>
+            tryif is_evar c
+            then (Util.Tac.build_term c ltac:(fun _ => left; solve [split]); commit_parents_B ps)
+            else idtac
+        | nil => idtac
+        end.
+
+      Ltac cancel_tr_opt_A c :=
+        lazymatch c with
+        | None    => idtac
+        | Some ?c => unify c false
+        end.
+
+      Ltac cancel_tr_opt_B c :=
+        lazymatch c with
+        | None                => idtac
+        | Some (mk_cb _ _ ?c) => Util.Tac.build_term c ltac:(fun _ => right; solve [split])
+        end.
+
+      Ltac mark_A n sA :=
+        lazymatch sA with
+        | @StAFirst ?a  ?w => unify w (WitAAtom n a)
+        | StATrf    ?n' ?c => unify n' n; cancel_tr_opt_A c
+        end.
+
+      Ltac mark_B sB :=
+        lazymatch sB with
+        | @StBFirst ?a ?w => unify w (WitBAtom a)
+        | StBTrf    ?c    => cancel_tr_opt_B c
+        end.
+
+      Ltac clear_A sA :=
+        lazymatch sA with
+        | @StAFirst ?a ?w  =>
+            unify w (WitAAtom ord_None a)
+        | StATrf ?n ?c =>
+            unify n ord_None;
+            cancel_tr_opt_A c
+        end.
+
+      Ltac clear_B sB :=
+        lazymatch sB with
+        | @StBFirst ?a ?w  =>
+            unify w (WitBAtom a)
+        | StBTrf ?c =>
+            cancel_tr_opt_B c
+        end.
+
+      Ltac clean_hyps :=
+        repeat lazymatch goal with
+        | H : A _ (StATrf ?n (Some true)) _ |- _ =>
+            unify n ord_None;
+            clear H
+        | H : B _ _ (StBTrf (Some (mk_cb _ _ (left _)))) _ |- _ =>
+            clear H
+        | H : A _   ?sA (false :: _) |- _ =>
+            clear_A sA;
+            clear H
+        | H : B _ _ ?sB (mk_cb _ _ (right _) :: _) |- _ =>
+            clear_B sB;
+            clear H
+        end.
+
+
+      Ltac match_hyps :=
+        lazymatch reverse goal with
+        | HB : B (existT _ ?v ?slB) ?n ?sB ?pB, HA : A (existT _ ?v ?slA) ?sA ?pA |- _ =>
+            (* idtac "MATCH" v; *)
+            unify slB slA;
+            mark_A (ord_of_r n) sA;
+            mark_B sB;
+            commit_parents_A pA;
+            commit_parents_B pB;
+            clear HA HB;
+            clean_hyps;
+            match_hyps
+        | _ => idtac
+        end.
+
+      (* reverts the hypotheses [StAFirst] and [StBFirst] *)
+      Lemma forall_to_arrow [A : Type] [B0 : A -> Type] [B1 : Type]
+        (E : forall x : A, B0 x = B1)
+        (C : A -> B1):
+        forall x : A, B0 x.
+      Proof.
+        intro x; rewrite E; apply (C x).
+      Qed.
+
+      Ltac revert_hyps_first fl :=
+        lazymatch goal with
+        | H : A _   (StAFirst _) _ |- _ => idtac
+        | H : B _ _ (StBFirst _) _ |- _ => idtac
+        | _ => fl tt
+        end;
+        repeat (
+          lazymatch goal with
+          | H : A _   (StAFirst _) _ |- _ => revert H
+          | H : B _ _ (StBFirst _) _ |- _ => revert H
+          end;
+          simple refine (forall_to_arrow _ _); [shelve|reflexivity|]
+        ).
+
+      (* try to apply transformations (auto intro/elim) *)
+      Lemma rewrite_elim_rule [rev a a' r]
+        (E : unfold_rule a a')
+        (C : elim_rule rev a' r):
+        elim_rule rev a r.
+      Proof.
+        rewrite E. exact C.
+      Qed.
+
+      Lemma apply_trf_A (a : atom) (w : wit_A a) (ps : list bool)
+        [rev : bool] [r : CTX.t]
+        (T : elim_rule rev a r)
+        [n : ord_t] [committed : bool] (G : Type)
+        (C : A a (StATrf n (Some committed)) ps -> intro_wit_A (committed :: ps) G r)
+        (W : w = if committed
+                 then @WitATrf rev a r T (fst (wit_of_intro_A (C (mk_A _ _ _))))
+                 else @WitAAtom n a)
+        (H : A a (StAFirst w) ps): G.
+      Proof.
+        apply (wit_of_intro_A (C (mk_A _ _ _))).
+      Qed.
+
+      Lemma no_trf_A (a : atom) (w : wit_A a) (ps : list bool)
+        (G : Type)
+        [n : ord_t]
+        (C : A a (StATrf n None) ps -> G)
+        (W : w = WitAAtom n a)
+        (H : A a (StAFirst w) ps) : G.
+      Proof.
+        apply C; constructor.
+      Qed.
+
+      Lemma rewrite_intro_rule [rev a a' r PT PF]
+        (E : unfold_rule a a')
+        (C : intro_rule rev a' r PT PF):
+        intro_rule rev a r PT PF.
+      Proof.
+        rewrite E. exact C.
+      Qed.
+
+      Lemma apply_trf_B (a : atom) (n : rord_t) (w : wit_B a) (ps : list committed_B_t)
+        [rev : bool] [r : CTX.t] [PT PF : Prop]
+        (T : intro_rule rev a r PT PF)
+        [committed : {PT}+{PF}] (G : Type)
+        (C : B a n (StBTrf (Some (mk_cb PT PF committed))) ps ->
+             intro_wit_B (mk_cb PT PF committed :: ps) O n G r)
+        (W : w = match committed with
+                 | left pf => @WitBTrf rev a r (get_intro_rule T pf)
+                                               (fst (wit_of_intro_B (C (mk_B _ _ _ _))))
+                 | right _ => @WitBAtom a
+                 end)
+        (H : B a n (StBFirst w) ps): G.
+      Proof.
+        apply (wit_of_intro_B (C (mk_B _ _ _ _))).
+      Qed.
+
+      Lemma no_trf_B (a : atom) (n : rord_t) (ps : list committed_B_t)
+        (G : Type)
+        (C : B a n (StBTrf None) ps -> G)
+        (H : B a n (StBFirst (WitBAtom a)) ps): G.
+      Proof.
+        apply C; constructor.
+      Qed.
+
+      Ltac apply_trf slv rfl k :=
+        lazymatch goal with
+        | |- A ?a (StAFirst ?w) ?ps -> ?G =>
+            let Tr := fresh "Tr" in
+            tryif
+              unshelve epose proof (Tr := apply_trf_A a w ps _);
+              [ (* rev *) shelve | (* r *) shelve
+              | (* T *)
+                repeat (refine (rewrite_elim_rule _ _); [slv tt |]);
+                slv tt | ]
+            then (
+              simple refine (Tr _ _ G _ _); clear Tr;
+              [ (* n *) shelve | (* committed *) shelve
+              | (* C *) intro; intro_wit_goal; apply_trf slv rfl k
+              | (* W *) rfl tt ]
+            ) else (
+              simple refine (no_trf_A a w ps G _ _);
+              [ (* n *) shelve
+              | (* C *) intro; apply_trf slv rfl k
+              | (* W *) rfl tt ]
+            )
+        | |- B ?a ?n (StBFirst ?w) ?ps -> ?G =>
+            let Tr := fresh "Tr" in
+            tryif
+              unshelve epose proof (Tr := apply_trf_B a n w ps _);
+              [ (* rev *) shelve | (* r *) shelve | (* PT *) shelve | (* PF *) shelve
+              | (* T *)
+                repeat (refine (rewrite_intro_rule _ _); [slv tt | cbn]);
+                slv tt | ]
+            then (
+              simple refine (Tr _ G _ _); clear Tr;
+              [ (* committed *) shelve
+              | (* C *) intro; intro_wit_goal; apply_trf slv rfl k
+              | (* W *) rfl tt ]
+            ) else (
+              simple refine (no_trf_B a n ps G _);
+              intro; apply_trf slv rfl k
+            )
+        | |- True => k tt
+        end.
+
+      Ltac transform_hyps fl k :=
+        revert_hyps_first fl;
+        apply_trf ltac:(fun _ => solve [eauto 1 with CtxTrfDB nocore])
+                  ltac:(fun _ => reflexivity)
+                  k.
+
+      Ltac build_iter fuel try_end :=
+        match_hyps;
+        try_end ltac:(fun fl =>
+        lazymatch fuel with
+        | O    => idtac "Fuel limit reached"; fl tt
+        | S ?n => transform_hyps fl ltac:(fun _ =>
+                  build_iter n try_end)
+        end).
+
+      Local Ltac build_until try_end :=
+        intro_wit_goal;
+        build_iter 10 try_end.
+
+      (* solves a goal:
+           Trf.p [mka vp0' sel0'; ... ; mka vp9' sel9']
+                 [mka vp0 ?sel0 ; ... ; mka vp9 ?sel5 ]
+                 ?rev_f
+       *)
+      Ltac build_p_end k :=
+        lazymatch goal with
+        | H : B ?a _ _ _ |- _ => k ltac:(fun _ => fail "Trf.build: remaining B" a)
+        | H : A ?a _ _   |- _ => k ltac:(fun _ => fail "Trf.build: remaining A" a)
+        | _ => exact Logic.I
+        end.
+
+      Ltac build_p :=
+        simple refine (build_trf_lem _ _ _ _ _ _ _);
+        [ (* W *) build_until build_p_end
+        | shelve | shelve | (* EW *) Tac.cbn_refl 
+        | (* E *) Tac.cbn_refl ].
+
+      (* solves a goal:
+           Trf.t [mka vp0' sel0'; ... ; mka vp9' sel9']
+                 [mka vp0 ?sel0 ; ... ; mka vp9 ?sel5 ]
+       *)
+      Ltac build_t :=
+        eexists; build_p.
+
+      (* solves a goal:
+           itrf [mka vp0' sel0'; ... ; mka vp9' sel9']
+                [mka vp0 ?sel0 ; ... ; mka vp9 ?sel5 ]
+                ?add ?rev_f
+       *)
+      Ltac build_inj_p_end k :=
+        lazymatch goal with
+        | H : B ?a _ _ _ |- _ => k ltac:(fun _ => fail "Trf.build_inj: remaining B" a)
+        | _ =>
+            repeat lazymatch goal with
+            | H : A _ ?sA _ |- _ => clear_A sA; clear H
+            end;
+            exact Logic.I
+        end.
+
+      Ltac build_inj_p :=
+        simple refine (build_inj_lem _ _ _ _ _ _ _ _);
+        [ (* W *) build_until build_inj_p_end
+        | shelve | shelve | (* EW *) Tac.cbn_refl
+        | (* E *) Tac.cbn_refl ].
+
+
+      Section Test.
+        Variable v : nat -> Vprop.p nat.
+
+        Goal exists sl0 sl1 rev_f,
+          Trf.p [mka (v 0, 0); mka (v 1, 1)] [mka (v 0, sl0); mka (v 1, sl1)] rev_f.
+        Proof.
+          do 3 eexists.
+          build_p.
+        Qed.
+
+        Goal exists sl0 sl1,
+          inhabited (Trf.t [mka (v 0, 0); mka (v 1, 1)] [mka (v 0, sl0); mka (v 1, sl1)]).
+        Proof.
+          do 3 eexists.
+          build_t.
+        Qed.
+
+        Goal exists sl0 sl1 add rev_f,
+          Trf.inj_p [mka (v 1, 1); mka (v 2, 2); mka (v 0, 0)] [mka (v 0, sl0); mka (v 1, sl1)] 
+            add rev_f.
+        Proof.
+          do 4 eexists.
+          build_inj_p.
+        Qed.
+
+
+        Variable w : Vprop.p (nat * nat).
+
+        Hypothesis W_elim  : forall sel, atomt false [mka (w, sel)] [mka (v 0, fst sel); mka (v 1, snd sel)].
+        Hypothesis W_intro : forall sl0 sl1, atomt true [mka (v 0, sl0); mka (v 1, sl1)] [mka (w, (sl0, sl1))] .
+
+        Definition W_lem_elim : forall sel,
+          elim_rule _ (existT _ {| Vprop.sl := w |} sel) _ := W_elim.
+        Lemma W_lem_intro sel sl0 sl1:
+          intro_rule true (existT _ {| Vprop.sl := w |} sel) [mka (v 0, sl0); mka (v 1, sl1)]
+            (sel = (sl0, sl1)) ((sl0, sl1) = (fst sel, snd sel)).
+        Proof.
+          constructor; intros ->.
+          apply W_intro.
+        Qed.
+
+        Local Hint Resolve W_lem_elim  | 1 : CtxTrfDB.
+        Local Hint Extern 1 (intro_rule _ (existT _ {| Vprop.sl := w |} _) _ _ _) =>
+          eapply W_lem_intro : CtxTrfDB.
+
+        Goal forall sl01, exists sl0 sl1 sl2 rev_f,
+          Trf.p [mka (w, sl01); mka (v 2, 2)] [mka (v 0, sl0); mka (v 1, sl1); mka (v 2, sl2)] rev_f.
+        Proof.
+          do 4 eexists.
+          build_p.
+        Qed.
+        
+        Goal forall sl01, exists sl0 sl1 add rev_f,
+          Trf.inj_p [mka (w, sl01); mka (v 2, 2)] [mka (v 0, sl0); mka (v 1, sl1)] add rev_f.
+        Proof.
+          do 4 eexists.
+          build_inj_p.
+        Qed.
+
+        Goal exists sl,
+          inhabited (Trf.t [mka (v 0, 0); mka (v 1, 1)] [mka (w, sl)]).
+        Proof.
+          do 2 eexists.
+          build_t.
+        Qed.
+
+        Variable w' : Vprop.p (nat * nat).
+        Hypothesis W'_eq : forall sel, SLprop.eq (sl [mka (w', sel)]) (sl [mka (w, sel)]).
+        Definition W'_lem_elim : forall sel,
+          elim_rule true (existT _ {| Vprop.sl := w' |} sel) _ := W'_eq.
+        Local Hint Resolve W'_lem_elim | 1 : CtxTrfDB.
+
+        Goal forall sl0, exists sl1 rev_f,
+          Trf.p [mka (w', sl0)] [mka (w, sl1)] rev_f /\
+          Tac.display (rev_f (Vector.cons _ true _ (Vector.nil _))).
+        Proof.
+          do 3 eexists.
+          build_p.
+          cbn.
+          reflexivity.
+        Qed.
+      End Test.
+    End Tac.
+  End Trf.
 End CTX.
 
 Module VpropList.
@@ -623,4 +1208,51 @@ Module VpropList.
     VpropList.of_ctx (c0 ++ c1) = VpropList.of_ctx c0 ++ VpropList.of_ctx c1
     := List.Transp.map_app _ c0 c1.
 End VpropList.
+
+Module Notations.
+  Notation "x ~> v" := (existT Vprop.ty (Vprop.mk x) v) (at level 100).
+  Notation "x ~>"   := (Vprop.mk x) (at level 100).
+  Definition vptr := SLprop.cell.
+  Global Arguments vptr/.
+End Notations.
+Import Notations.
+
+Module VRecord.
+  Inductive p (A : Type) (vs : VpropList.t)
+    (f : A -> Tuple.u_t (VpropList.sel vs))
+    (g : Tuple.arrow (VpropList.sel vs) (fun _ => A))
+    : Prop
+  := mk_p (GF : Tuple.arrow (VpropList.sel vs) (fun sl1 => Tuple.of_u_t (f (Tuple.to_fun g sl1)) = sl1)).
+
+  Definition v [A vs f g] (P : p A vs f g) : Vprop.p A :=
+    fun x => CTX.sl (VpropList.inst vs (Tuple.of_u_t (f x))).
+
+  Lemma elim_rule [A vs f g] (P : p A vs f g) sl:
+    CTX.Trf.Tac.elim_rule true
+      (VRecord.v P ~> sl) (VpropList.inst vs (Tuple.of_u_t (f sl))).
+  Proof.
+    unfold VRecord.v; cbn; SL.normalize.
+    reflexivity.
+  Qed.
+
+  Lemma intro_rule [A vs f g] (P : p A vs f g) sl0 sl1 :
+    CTX.Trf.Tac.intro_rule true
+      (VRecord.v P ~> sl0) (VpropList.inst vs sl1)
+      (sl0 = Tuple.to_fun g sl1) (sl1 = Tuple.of_u_t (f sl0)).
+  Proof.
+    constructor; intros ->; unfold v; cbn; SL.normalize.
+    ecase P as [->%Tuple.to_fun].
+    reflexivity.
+  Qed.
+
+  Ltac intro_rule_tac A vs f g P sl0 :=
+    simple refine (@intro_rule A vs f g P sl0 _);
+    Tuple.build_shape (* sl1 *).
+
+  Module Tactics.
+    #[export] Hint Resolve VRecord.elim_rule | 1 : CtxTrfDB.
+    #[export] Hint Extern 1 (CTX.Trf.Tac.intro_rule _ (@VRecord.v ?A ?vs ?f ?g ?P ~> ?sl0) _ _ _) =>
+      VRecord.intro_rule_tac A vs f g P sl0 : CtxTrfDB.
+  End Tactics.
+End VRecord.
 
